Prove reorder instr; fence

src/trans/ReorderFence.v
@@ -22,6 +22,7 @@ Require Import Thread.
 Require Import Configuration.
 
 Require Import Progress.
+Require Import ReorderInternal.
 
 Require Import SimLocal.
 Require Import SimMemory.
@@ -37,7 +38,7 @@ Require Import ITreeLib.
 Set Implicit Arguments.
 
 
-Inductive reorder_fence (or1 ow1:Ordering.t): forall R (i2:MemE.t R), Prop :=
+Variant reorder_fence (or1 ow1:Ordering.t): forall R (i2:MemE.t R), Prop :=
 | reorder_fence_load
     l2 o2
     (ORDR1: Ordering.le or1 Ordering.acqrel)
@@ -58,21 +59,26 @@ Inductive reorder_fence (or1 ow1:Ordering.t): forall R (i2:MemE.t R), Prop :=
     reorder_fence or1 ow1 (MemE.update l2 rmw2 or2 ow2)
 .
 
-Inductive sim_fence: forall R
-                            (st_src:itree MemE.t (unit * R)%type) (lc_src:Local.t) (sc1_src:TimeMap.t) (mem1_src:Memory.t)
-                            (st_tgt:itree MemE.t (unit * R)%type) (lc_tgt:Local.t) (sc1_tgt:TimeMap.t) (mem1_tgt:Memory.t), Prop :=
+Variant sim_fence: forall R
+                            (st_src:itree MemE.t (unit * R)%type) (lc_src:Local.t) (gl1_src:Global.t)
+                            (st_tgt:itree MemE.t (unit * R)%type) (lc_tgt:Local.t) (gl1_tgt:Global.t), Prop :=
 | sim_fence_intro
     R
     or1 ow1 (i2: MemE.t R)
-    lc1_src sc1_src mem1_src
-    lc1_tgt sc1_tgt mem1_tgt
-    lc2_src sc2_src
+    lc1_src gl1_src
+    lc1_tgt gl1_tgt
+    lc2_src gl2_src
     (REORDER: reorder_fence or1 ow1 i2)
-    (FENCE: Local.fence_step lc1_src sc1_src or1 ow1 lc2_src sc2_src)
-    (LOCAL: sim_local SimPromises.bot lc2_src lc1_tgt):
+    (FENCE: Local.fence_step lc1_src gl1_src or1 ow1 lc2_src gl2_src)
+    (LOCAL: sim_local lc2_src lc1_tgt)
+    (GLOBAL: sim_global gl1_src gl1_tgt)
+    (LC_WF_SRC: Local.wf lc1_src gl1_src)
+    (LC_WF_TGT: Local.wf lc1_tgt gl1_tgt)
+    (GL_WF_SRC: Global.wf gl1_src)
+    (GL_WF_TGT: Global.wf gl1_tgt):
     sim_fence
-      (Vis i2 (fun v2 => Vis (MemE.fence or1 ow1) (fun v1 => Ret (v1, v2)))) lc1_src sc1_src mem1_src
-      (Vis i2 (fun r => Ret (tt, r))) lc1_tgt sc1_tgt mem1_tgt
+      (Vis i2 (fun v2 => Vis (MemE.fence or1 ow1) (fun v1 => Ret (v1, v2)))) lc1_src gl1_src
+      (Vis i2 (fun r => Ret (tt, r))) lc1_tgt gl1_tgt
 .
 
 Lemma read_fence_wf
@@ -83,174 +89,177 @@ Proof.
   inv WF. econs; ss; condtac; eauto. refl.
 Qed.
 
+Lemma fence_step_non_sc
+      lc1 gl1 or ow lc2 gl2
+      (STEP: Local.fence_step lc1 gl1 or ow lc2 gl2)
+      (SC: Ordering.le ow Ordering.acqrel):
+  gl2 = gl1.
+Proof.
+  destruct gl1. inv STEP. ss. f_equal.
+  apply TViewFacts.write_fence_sc_acqrel. ss.
+Qed.
+
+Lemma sim_fence_mon
+      R
+      st_src lc_src gl1_src
+      st_tgt lc_tgt gl1_tgt
+      gl2_src
+      gl2_tgt
+      (SIM1: sim_fence st_src lc_src gl1_src
+                       st_tgt lc_tgt gl1_tgt)
+      (GL_LE_SRC: Global.le gl1_src gl2_src)
+      (GL_LE_TGT: Global.le gl1_tgt gl2_tgt)
+      (GLOBAL1: sim_global gl2_src gl2_tgt)
+      (LC_WF_SRC: Local.wf lc_src gl2_src)
+      (LC_WF_TGT: Local.wf lc_tgt gl2_tgt)
+      (GL_WF_SRC: Global.wf gl2_src)
+      (GL_WF_TGT: Global.wf gl2_tgt):
+  @sim_fence R
+             st_src lc_src gl2_src
+             st_tgt lc_tgt gl2_tgt.
+Proof.
+  dependent destruction SIM1.
+  exploit future_fence_step; try exact FENCE; try apply GL_LE_SRC; eauto.
+  { inv REORDER; destruct ow1; ss. }
+  i. econs; eauto.
+Qed.
+
 Lemma sim_fence_sim_local
       R
-      st_src lc_src sc_src mem_src
-      st_tgt lc_tgt sc_tgt mem_tgt
-      (WF_SRC: TView.wf lc_src.(Local.tview))
-      (SIM: @sim_fence R st_src lc_src sc_src mem_src st_tgt lc_tgt sc_tgt mem_tgt):
-  sim_local SimPromises.bot lc_src lc_tgt.
+      st_src lc_src gl_src
+      st_tgt lc_tgt gl_tgt
+      (SIM: @sim_fence R st_src lc_src gl_src st_tgt lc_tgt gl_tgt):
+  sim_local lc_src lc_tgt.
 Proof.
   inv SIM. inv FENCE. inv LOCAL. ss.
   econs; eauto. etrans; eauto.
   etrans; cycle 1.
   { eapply TViewFacts.write_fence_tview_incr.
-    eapply read_fence_wf; eauto.
+    eapply read_fence_wf; eauto. apply LC_WF_SRC.
   }
-  eapply TViewFacts.read_fence_tview_incr. apply WF_SRC.
+  eapply TViewFacts.read_fence_tview_incr. apply LC_WF_SRC.
 Qed.
 
 Lemma sim_fence_step
       R
-      st1_src lc1_src sc0_src mem0_src
-      st1_tgt lc1_tgt sc0_tgt mem0_tgt
-      (SIM: sim_fence st1_src lc1_src sc0_src mem0_src
-                      st1_tgt lc1_tgt sc0_tgt mem0_tgt):
-  forall sc1_src sc1_tgt
-    mem1_src mem1_tgt
-    (SC: TimeMap.le sc1_src sc1_tgt)
-    (MEMORY: sim_memory mem1_src mem1_tgt)
-    (SC_FUTURE_SRC: TimeMap.le sc0_src sc1_src)
-    (SC_FUTURE_TGT: TimeMap.le sc0_tgt sc1_tgt)
-    (MEM_FUTURE_SRC: Memory.future_weak mem0_src mem1_src)
-    (MEM_FUTURE_TGT: Memory.future_weak mem0_tgt mem1_tgt)
-    (WF_SRC: Local.wf lc1_src mem1_src)
-    (WF_TGT: Local.wf lc1_tgt mem1_tgt)
-    (SC_SRC: Memory.closed_timemap sc1_src mem1_src)
-    (SC_TGT: Memory.closed_timemap sc1_tgt mem1_tgt)
-    (MEM_SRC: Memory.closed mem1_src)
-    (MEM_TGT: Memory.closed mem1_tgt),
+      st1_src lc1_src gl1_src
+      st1_tgt lc1_tgt gl1_tgt
+      (SIM: sim_fence st1_src lc1_src gl1_src
+                      st1_tgt lc1_tgt gl1_tgt):
   _sim_thread_step (lang (unit * R)%type) (lang (unit * R)%type)
-                   ((@sim_thread (lang (unit * R)%type) (lang (unit * R)%type) (sim_terminal eq)) \8/ @sim_fence R)
-                     st1_src lc1_src sc1_src mem1_src
-                     st1_tgt lc1_tgt sc1_tgt mem1_tgt.
+                   ((@sim_thread (lang (unit * R)%type) (lang (unit * R)%type) (sim_terminal eq)) \6/ @sim_fence R)
+                     st1_src lc1_src gl1_src
+                     st1_tgt lc1_tgt gl1_tgt.
 Proof.
-  i. exploit sim_fence_sim_local; eauto; try apply WF_SRC. intro SIM_LC.
+  exploit sim_fence_sim_local; eauto; try apply WF_SRC. intro SIM_LC.
   destruct SIM. ii.
-  exploit future_fence_step; try apply FENCE; eauto; i.
-  { inv REORDER; etrans; eauto. }
-  inv STEP_TGT; [inv STEP|dependent destruction STEP; inv LOCAL0; ss; dependent destruction STATE; inv REORDER]; ss.
-  - (* promise *)
+  assert (OW: Ordering.le ow1 Ordering.acqrel)
+    by (inv FENCE; inv REORDER; destruct ow1; ss).
+  exploit Local.fence_step_future; eauto. i. des.
+  exploit fence_step_non_sc; try exact FENCE; ss. i. subst.
+  inv STEP_TGT; ss.
+  { (* internal *)
     right.
-    exploit sim_local_promise; try exact LOCAL; eauto.
-    { eapply Local.fence_step_future; eauto. }
-    i. des.
-    exploit reorder_fence_promise; try apply x0; try apply STEP_SRC; eauto.
-    { inv REORDER; ss. }
-    i. des.
-    esplits; try apply SC; eauto; ss.
-    + econs 2. econs 1. econs; eauto.
-    + eauto.
+    exploit Local.internal_step_future; eauto. i. des.
+    exploit sim_local_internal; try exact LOCAL; eauto. i. des.
+    exploit reorder_fence_internal; try exact FENCE; try exact STEP_SRC; eauto. i. des.
+    exploit Local.internal_step_future; eauto. i. des.
+    exploit fence_step_non_sc; try exact STEP2; eauto. i. subst.
+    esplits; try apply GL2; eauto; ss.
+    + inv LOCAL0; ss.
     + right. econs; eauto.
+  }
+  inv LOCAL0; ss; dependent destruction REORDER; dependent destruction STATE.
   - (* load *)
     right.
     guardH ORD2.
-    exploit sim_local_read; try exact LOCAL0; try exact LOCAL; try apply SC; eauto; try refl; viewtac.
-    { eapply Local.fence_step_future; eauto. }
-    i. des.
-    exploit reorder_fence_read; try apply x0; try apply STEP_SRC; eauto; try by viewtac. i. des.
+    exploit sim_local_read; try exact LOCAL1; try exact LOCAL; eauto; try refl. i. des.
+    exploit reorder_fence_read; try exact FENCE; try exact STEP_SRC; eauto. i. des.
     esplits.
     + ss.
     + econs 2; [|econs 1]. econs.
-      * econs. econs 2. econs; [|econs 2]; eauto. econs. econs.
-      * eauto.
-    + econs 2. econs 2. econs; [|econs 5]; eauto. econs. econs.
-    + auto.
+      * econs 2; [|econs 2]; eauto. econs. refl.
+      * ss.
+    + econs 2. econs 2; [|econs 5]; eauto. econs. refl.
+    + ss.
     + etrans; eauto.
-    + auto.
-    + left. eapply paco11_mon; [apply sim_itree_ret|]; ss.
-      etrans; eauto.
+    + left. eapply paco9_mon; [apply sim_itree_ret|]; ss. etrans; eauto.
   - (* update-load *)
     right.
     guardH ORDR2.
-    exploit sim_local_read; try exact LOCAL0; try exact LOCAL; try apply SC; eauto; try refl; viewtac.
-    { eapply Local.fence_step_future; eauto. }
-    i. des.
-    exploit reorder_fence_read; try apply x0; try apply STEP_SRC; eauto; try by viewtac. i. des.
+    exploit sim_local_read; try exact LOCAL1; try exact LOCAL; eauto; try refl. i. des.
+    exploit reorder_fence_read; try exact FENCE; try exact STEP_SRC; eauto. i. des.
     esplits.
     + ss.
     + econs 2; [|econs 1]. econs.
-      * econs. econs 2. econs; [|econs 2]; eauto. econs; eauto.
-      * eauto.
-    + econs 2. econs 2. econs; [|econs 5]; eauto. econs. econs.
-    + auto.
+      * econs 2; [|econs 2]; eauto. econs; eauto.
+      * ss.
+    + econs 2. econs 2; [|econs 5]; eauto. econs. refl.
+    + ss.
     + etrans; eauto.
-    + auto.
-    + left. eapply paco11_mon; [apply sim_itree_ret|]; ss.
-      etrans; eauto.
+    + left. eapply paco9_mon; [apply sim_itree_ret|]; ss. etrans; eauto.
   - (* store *)
     right.
-    hexploit sim_local_write_bot; try exact LOCAL1; try exact LOCAL; try apply SC;
+    hexploit sim_local_write; try exact LOCAL1; try exact LOCAL;
       try match goal with
           | [|- is_true (Ordering.le _ _)] => refl
-          end; eauto; try refl; viewtac.
-    { eapply Local.fence_step_future; eauto. }
+          end; eauto; try refl.
     i. des.
-    exploit reorder_fence_write; try apply x0; try apply STEP_SRC; eauto; try by viewtac. i. des.
+    exploit reorder_fence_write; try apply FENCE; try apply STEP_SRC; eauto. i. des.
     esplits.
     + ss.
     + econs 2; [|econs 1]. econs.
-      * econs. econs 2. econs; [|econs 3]; eauto. econs. econs.
-      * eauto.
-    + econs 2. econs 2. econs; [|econs 5]; eauto. econs. econs.
-    + auto.
+      * econs 2; [|econs 3]; eauto. econs. refl.
+      * ss.
+    + econs 2. econs 2; [|econs 5]; eauto. econs. refl.
+    + ss.
     + etrans; eauto.
-    + etrans; eauto.
-    + left. eapply paco11_mon; [apply sim_itree_ret|]; ss.
-      etrans; eauto.
+    + left. eapply paco9_mon; [apply sim_itree_ret|]; ss. etrans; eauto.
   - (* update *)
     right.
     guardH ORDR2.
     exploit Local.read_step_future; eauto. i. des.
-    exploit sim_local_read; try exact LOCAL1; try exact LOCAL; try apply SC; eauto; try refl; viewtac.
-    { eapply Local.fence_step_future; eauto. }
-    i. des.
-    exploit reorder_fence_read; try apply x0; try apply STEP_SRC; eauto; try by viewtac. i. des.
+    exploit sim_local_read; try exact LOCAL1; try exact LOCAL; eauto; try refl. i. des.
+    exploit reorder_fence_read; try apply FENCE; try apply STEP_SRC; eauto. i. des.
     exploit Local.read_step_future; eauto. i. des.
     exploit Local.fence_step_future; eauto. i. des.
     generalize LOCAL3. i. rewrite LOCAL0 in LOCAL3.
-    generalize SC0. i. rewrite SC in SC1.
-    hexploit sim_local_write_bot; try exact LOCAL2; try apply SC1; eauto; try refl; viewtac. i. des.
-    exploit reorder_fence_write; try apply STEP2; try apply STEP_SRC0; eauto; try by viewtac. i. des.
+    generalize GLOBAL0. i. rewrite GLOBAL in GLOBAL0.
+    hexploit sim_local_write; try exact LOCAL2; try exact GLOBAL1; eauto; try refl. i. des.
+    exploit reorder_fence_write; try apply STEP2; try apply STEP_SRC0; eauto. i. des.
     esplits.
     + ss.
     + econs 2; [|econs 1]. econs.
-      * econs. econs 2. econs; [|econs 4]; eauto. econs; eauto.
-      * eauto.
-    + econs 2. econs 2. econs; [|econs 5]; eauto. econs. econs.
-    + auto.
+      * econs 2; [|econs 4]; eauto. econs; eauto.
+      * ss.
+    + econs 2. econs 2; [|econs 5]; eauto. econs. refl.
+    + ss.
     + etrans; eauto.
-    + etrans; eauto.
-    + left. eapply paco11_mon; [apply sim_itree_ret|]; ss.
-      etrans; eauto.
-  - (* na write *)
-    inv LOCAL1. destruct ord; ss.
+    + left. eapply paco9_mon; [apply sim_itree_ret|]; ss. etrans; eauto.
   - (* racy read *)
     right. guardH ORD2.
-    exploit sim_local_racy_read; try exact SIM_LC; eauto; try refl. i. des.
+    exploit sim_local_racy_read; try exact LOCAL1; eauto; try refl. i. des.
     esplits.
     + ss.
     + econs 2; [|econs 1]. econs.
-      * econs. econs 2. econs; [|econs 9]; eauto. econs. econs.
-      * eauto.
-    + econs 2. econs 2. econs; [|econs 5]; eauto. econs. econs.
-    + auto.
+      * econs 2; [|econs 8]; eauto. econs. refl.
+      * ss.
+    + econs 2. econs 2; [|econs 5]; eauto. econs. refl.
     + ss.
     + ss.
-    + left. eapply paco11_mon; [apply sim_itree_ret|]; ss.
+    + left. eapply paco9_mon; [apply sim_itree_ret|]; ss.
   - (* racy read *)
     right. guardH ORDR2.
-    exploit sim_local_racy_read; try exact SIM_LC; eauto; try refl. i. des.
+    exploit sim_local_racy_read; try exact LOCAL1; eauto; try refl. i. des.
     esplits.
     + ss.
     + econs 2; [|econs 1]. econs.
-      * econs. econs 2. econs; [|econs 9]; eauto. econs; eauto.
-      * eauto.
-    + econs 2. econs 2. econs; [|econs 5]; eauto. econs. econs.
-    + auto.
+      * econs 2; [|econs 8]; eauto. econs; eauto.
+      * ss.
+    + econs 2. econs 2; [|econs 5]; eauto. econs. refl.
     + ss.
     + ss.
-    + left. eapply paco11_mon; [apply sim_itree_ret|]; ss.
+    + left. eapply paco9_mon; [apply sim_itree_ret|]; ss.
   - (* racy write *)
     left.
     exploit sim_local_racy_write; try exact LOCAL1; try exact SIM_LC;
@@ -258,8 +267,8 @@ Proof.
           | [|- is_true (Ordering.le _ _)] => refl
           end; eauto.
     i. des.
-    unfold Thread.steps_failure. esplits; try refl.
-    + econs 2. econs; [|econs 10]; eauto. econs. econs.
+    econs; try refl.
+    + econs 2; [|econs 9]; eauto. econs. refl.
     + ss.
   - (* racy update *)
     left. guardH ORDR2.
@@ -268,21 +277,21 @@ Proof.
           | [|- is_true (Ordering.le _ _)] => refl
           end; eauto.
     i. des.
-    unfold Thread.steps_failure. esplits; try refl.
-    + econs 2. econs; [|econs 11]; eauto. econs; eauto.
+    econs; try refl.
+    + econs 2; [|econs 10]; eauto. econs; eauto.
     + ss.
 Qed.
 
 Lemma sim_fence_sim_thread R:
-  @sim_fence R <8= @sim_thread (lang (unit * R)%type) (lang (unit * R)%type) (sim_terminal eq).
+  @sim_fence R <6= @sim_thread (lang (unit * R)%type) (lang (unit * R)%type) (sim_terminal eq).
 Proof.
   pcofix CIH. i. pfold. ii. ss. splits; ss; ii.
   - right. inv TERMINAL_TGT. inv PR; ss.
   - right. esplits; eauto.
-    inv PR. inversion FENCE. subst lc2_src. inversion LOCAL. ss.
-    apply SimPromises.sem_bot_inv in PROMISES0; auto. rewrite PROMISES0. auto.
-  - exploit sim_fence_step; try apply PR; try apply SC; eauto. i. des; eauto.
+    inv PR. inv FENCE. inv LOCAL. ss. congr.
+  - exploit sim_fence_mon; eauto; try apply GL_FUTURE_SRC. i.
+    exploit sim_fence_step; try exact x0; eauto. i. des; eauto.
     + right. esplits; eauto.
-      left. eapply paco11_mon; eauto. ss.
+      left. eapply paco9_mon; eauto. ss.
     + right. esplits; eauto.
 Qed.
